FMapList.v
@@ -19,104 +19,13 @@ Require Import FMapInterface.
 
 Set Implicit Arguments.
 Unset Strict Implicit.
-Implicit Arguments equivalence.
-Implicit Arguments order.
-Implicit Arguments reflexive.
-Implicit Arguments transitive.
-Implicit Arguments symmetric.
-Implicit Arguments antisymmetric.
 
 (** Usual syntax for lists. *)
 Notation "[]" := nil (at level 0).
 
-(*
-Module PairLeftOrderedType(X:OrderedType).
-
-  Module E := X. (* À quoi cela sert-il? *)
-  Module ME := OrderedTypeFacts X.
-  Definition key := X.t.
-    
-  Section Elt.
-    Variable elt:Set.
-    Variable eq_elt:elt -> elt -> Prop.
-    Variable eq_elt_equiv:equivalence eq_elt.
-
-    Hint Resolve (equiv_refl _ _ eq_elt_equiv) (equiv_trans _ _ eq_elt_equiv)
-      .
-
-    Definition t := (key*elt)%type.
-
-    Definition eq (c1 c2: key * elt):Prop :=
-      let (x,y) := c1 in let (x',y') := c2 in  E.eq x x' /\ eq_elt y y'.
-
-    Definition eq_key (c1 c2: key * elt):Prop :=
-      let (x,y) := c1 in let (x',y') := c2 in  E.eq x x'.
-
-    Definition lt (c1 c2: key * elt):Prop :=
-      let (x,y) := c1 in let (x',y') := c2 in  E.lt x x'.
-
-
-    Lemma eq_eq_key : forall e e', eq e e' -> eq_key e e'.
-      intros e e'.
-      case e. case e'. simpl.
-      intros k e0 k0 e1 hyp.
-      decompose [and] hyp;auto. 
-      (* do not use intuition here, because it produces a dependency on
-         eq_elt_equiv above*)
-    Qed.
-
-    Lemma eq_refl : forall e, eq e e.
-      intro e. case e;simpl; auto.
-    Qed.
-
-    Lemma eq_key_refl : forall e, eq_key e e.
-      intro e. case e;simpl; auto.
-    Qed.
-
-    Lemma eq_sym : forall e e', eq_key e e' -> eq_key e' e.
-      intros e e'. case e. case e'. simpl. intuition.
-    Qed.
-
-    Lemma eq_key_sym : forall e e', eq_key e e' -> eq_key e' e.
-      intros e e'. case e. case e'. simpl;intuition.
-    Qed.
-
-    Lemma eq_trans : forall e e' e'', eq e e' -> eq e' e'' -> eq e e''.
-      intros e e' e''. case e. case e'. case e''. simpl;intuition;eauto.
-    Qed.
-
-    Lemma eq_key_trans : forall e e' e'', eq_key e e' -> eq_key e' e'' -> eq_key e e''.
-      intros e e' e''. case e. case e'. case e''. simpl;intuition;eauto.
-    Qed.
-
-    Lemma lt_not_eq : forall e e', lt e e' -> ~eq e e'.
-      intros e e'. case e. case e'. simpl.
-      intros k e0 k0 e1 H.
-      intro abs;destruct abs.
-      elim (E.lt_not_eq H); assumption.
-    Qed.
-
-    Lemma lt_not_eq_key : forall e e', lt e e' -> ~eq_key e e'.
-      intros e e'. case e. case e'. simpl.
-      intros k e0 k0 e1 H.
-      intro abs.
-      elim (E.lt_not_eq H); assumption.
-    Qed.
-
-    Lemma lt_trans : forall e e' e'', lt e e' -> lt e' e'' -> lt e e''.
-      intros e e' e''. case e. case e'. case e''. simpl;eauto.
-    Qed.
-
-  End Elt.
-End PairLeftOrderedType.
-*)
-
-
 Module Raw (X:OrderedType).
   Module E := X. (* À quoi cel sert-il? *)
   Module ME := OrderedTypeFacts X.
-
-(*  Module PE := PairLeftOrderedType X. *)
 
   Definition key := X.t.
   Arguments Scope list [type_scope].
@@ -135,9 +44,6 @@ Module Raw (X:OrderedType).
   Definition MapsTo (k:key)(e:elt):= InList eq_key_elt (k,e).
   Definition In k m := exists e:elt, MapsTo k e m.
   Definition Empty m := forall (a : key)(e:elt) , ~ MapsTo a e m.
-  Definition Equal m m' := forall (a : key) (e e': elt), 
-      (In a m <-> In a m') /\
-      (MapsTo a e m -> MapsTo a e' m' -> e = e'). 
 
   Lemma InList_eq_key_el_eq_key : 
       forall x m, InList eq_key_elt x m -> InList eq_key x m.
@@ -296,17 +202,6 @@ Module Raw (X:OrderedType).
 
     Hint Resolve all_lt_Inf.
 
-(*    Lemma sorted_hd_all_lt: forall x l e, 
-      Sort (x::l) -> InList eq_key_elt e l -> ltkey x e.
-      intros x l e sorted inl.
-      induction inl;eauto.
-      assert (ltkey x y);eauto.
-      inversion sorted.
-      inversion H3;auto.
-    Qed.
-
-    Hint Resolve sorted_hd_all_lt.
-*)
     Lemma sort_in_tl : forall e l e', Sort (e::l) -> InList eq_key e' l -> lt_key e e'.
       intros e l e' sorted Hin.
       induction Hin;eauto.
@@ -451,8 +346,7 @@ Module Raw (X:OrderedType).
       inversion inlist;auto.
     Qed.
 
-
-(** end of auxiliary results *)
+   (** end of auxiliary results *)
 
     Definition empty : t elt := [].
 
@@ -794,7 +688,6 @@ Module Raw (X:OrderedType).
 	decompose [and] hyp. clear hyp.
         exists ((k, e) ::x);intuition.
 
-(* 	apply sorted_unique. *)
 	apply cons_sort;auto.
 	assert (Inf (k, e) m').
 
@@ -845,6 +738,130 @@ Module Raw (X:OrderedType).
 	exists x;intuition;auto.
 	apply sorted_unique;auto.
       Qed.
+
+     Fixpoint equal (cmp: elt -> elt -> bool)(m m' : t elt) { struct m } : bool := 
+       match m, m' with 
+        | [], [] => true
+        | (x,e)::l, (x',e')::l' => 
+            match E.compare x x' with 
+             | Eq _ => cmp e e' && equal cmp l l'
+             | _       => false
+            end 
+        | _, _ => false 
+       end.
+
+     Definition Equal cmp m m' := 
+         (forall k, In k m <-> In k m') /\ 
+         (forall k e e', MapsTo k e m -> MapsTo k e' m' -> cmp e e' = true).  
+
+     (** Specification of [equal] *)
+        Lemma equal_1 : forall m (Hm:Sort m) m' (Hm': Sort m') cmp, 
+           Equal cmp m m' -> equal cmp m m' = true. 
+        Proof. 
+        intros m Hm m' Hm' cmp; generalize Hm Hm'; clear Hm Hm'.
+        functional induction equal cmp m m'; simpl; auto; unfold Equal; intuition.
+
+        destruct p as (k,e).
+        destruct (H0 k).
+        destruct H2; eauto.
+        inversion H2.
+
+        destruct (H0 x).
+        destruct H; eauto.
+        inversion H.
+
+        subst; clear H_eq_3.
+        destruct (H0 x).
+        assert (In x ((x',e')::l')). 
+          apply H; auto.
+          exists e; auto.
+        destruct (In_inv H3).
+        absurd (E.lt x x'); eauto.
+        inversion_clear Hm'.
+        assert (Inf (x,e) l').
+        eapply Inf_lt; eauto; auto. (* eauto n'est pas strictement plus fort que auto ??! *)
+        elim (sort_lt_notin H5 H7 H4).
+        
+        subst.
+        assert (cmp e e' = true).
+          apply H2 with x; auto.
+        rewrite H0; simpl.
+       apply H; auto.
+       inversion_clear Hm; auto.
+       inversion_clear Hm'; auto.
+       unfold Equal; intuition.
+       destruct (H1 k).
+       assert (In k ((x,e) ::l)).
+         destruct H3 as (e'', hyp); exists e''; auto.
+       destruct (In_inv (H4 H6)); auto.
+       inversion_clear Hm.
+       elim (sort_lt_notin H8 H9).
+       destruct H3 as (e'', hyp); exists e''; auto.
+       apply MapsTo_1 with k; eauto.
+       destruct (H1 k).
+       assert (In k ((x',e') ::l')).
+         destruct H3 as (e'', hyp); exists e''; auto.
+       destruct (In_inv (H5 H6)); auto.
+       inversion_clear Hm'.
+       elim (sort_lt_notin H8 H9).
+       destruct H3 as (e'', hyp); exists e''; auto.
+       apply MapsTo_1 with k; eauto.
+       apply H2 with k; destruct (ME.eq_dec x k); auto.
+
+        subst; clear H_eq_3.
+        destruct (H0 x').
+        assert (In x' ((x,e)::l)). 
+          apply H2; auto.
+          exists e'; auto.
+        destruct (In_inv H3).
+        absurd (E.lt x' x); eauto.
+        inversion_clear Hm.
+        assert (Inf (x',e') l).
+        eapply Inf_lt; eauto; auto. (* eauto n'est pas strictement plus fort que auto ??! *)
+        elim (sort_lt_notin H5 H7 H4).
+     Qed.
+
+      Lemma equal_2 : forall m (Hm:Sort m) m' (Hm:Sort m') cmp, 
+         equal cmp m m' = true -> Equal cmp m m'.
+      Proof.
+       intros m Hm m' Hm' cmp; generalize Hm Hm'; clear Hm Hm'.
+       functional induction equal cmp m m'; simpl; auto; unfold Equal; intuition; try discriminate; subst.
+       inversion H0.
+
+       destruct (andb_prop _ _ H0); clear H0.
+       inversion_clear Hm; inversion_clear Hm'.
+       destruct (H H0 H5 H3).
+       destruct (In_inv H1).
+       exists e'; eauto.
+       destruct (H7 k).
+       destruct (H10 H9) as (e'',hyp).
+       exists e''; eauto.
+
+       destruct (andb_prop _ _ H0); clear H0.
+       inversion_clear Hm; inversion_clear Hm'.
+       destruct (H H0 H5 H3).
+       destruct (In_inv H1).
+       exists e; eauto.
+       destruct (H7 k).
+       destruct (H11 H9) as (e'',hyp).
+       exists e''; eauto.
+
+       destruct (andb_prop _ _ H0); clear H0.
+       inversion_clear Hm; inversion_clear Hm'.
+       destruct (H H0 H6 H4).
+       inversion_clear H1.
+       dec_eq_key_elt; simpl in *; subst.
+       inversion_clear H2. 
+       dec_eq_key_elt; simpl in *; subst; auto.
+       elim (sort_lt_notin H6 H7).
+       exists e'0; apply MapsTo_1 with k; eauto.
+       inversion_clear H2. 
+       dec_eq_key_elt; simpl in *; subst; auto.
+       elim (sort_lt_notin H0 H5).
+       exists e1; apply MapsTo_1 with k; eauto.
+       apply H9 with k; eauto.
+      Qed. 
+      
 
       Variable elt':Set.
       
@@ -1023,10 +1040,12 @@ Module Make (X: OrderedType) <: S with Module E := X.
  Definition map f m : t elt' := Build_slist (Raw.map_sorted m.(sorted) f).
  Definition mapi f m : t elt' := Build_slist (Raw.mapi_sorted m.(sorted) f).
  Definition fold A f m i := @Raw.fold elt A f m.(this) i.
+ Definition equal cmp m m' := @Raw.equal elt cmp m.(this) m'.(this).
 
  Definition MapsTo x e m := Raw.MapsTo x e m.(this).
  Definition In x m := Raw.In x m.(this).
  Definition Empty m := Raw.Empty m.(this).
+ Definition Equal cmp m m' := @Raw.Equal elt cmp m.(this) m'.(this).
 
  Definition eq_key (p p':key*elt) := E.eq (fst p) (fst p').
      
@@ -1062,313 +1081,204 @@ Module Make (X: OrderedType) <: S with Module E := X.
  Definition mapi_1 m := @Raw.mapi_1 elt elt' m.(this).
  Definition mapi_2 m := @Raw.mapi_2 elt elt' m.(this).
 
- 
+ Definition equal_1 m m' := @Raw.equal_1 elt m.(this) m.(sorted) m'.(this) m'.(sorted).
+ Definition equal_2 m m' := @Raw.equal_2 elt m.(this) m.(sorted) m'.(this) m'.(sorted).
+
  End Elt.
-
-
 End Make.
 
 
-(* TO BE CONTINUED ....
 
-
-
-
-
-
-
-
- 
-    Definition eq := Equal.
-    
-    Inductive lt (ltelt: elt -> elt -> Prop) : t elt -> t elt -> Prop :=
-      | lt_nil : forall (k: key) (x : elt) (s : t elt), lt ltelt [] ((k,x) :: s)
-      | lt_cons_lt : 
-	forall k x k' y (s s' : t elt), 
-	  E.lt k k' -> lt ltelt ((k,x) :: s) ((k',y) :: s')
-      | lt_cons_eq_lt :
-        forall k x k' y (s s' : t elt), 
-	  E.eq k k' -> ltelt x y -> lt ltelt ((k,x) :: s) ((k',y) :: s').
-    Hint Constructors lt.
-
-
-
- 
-(* 
-    Definition compare (elt_eq:forall e e', Compare lt_elt (Logic.eq (A:=elt)) e e'): 
-      forall m m' : t elt, Compare (lt lt_elt) (eq eq_elt) m m'.
- *)
-
-
-(*
-  (** Very useful lemma. It means that if the list of pairs is sorted, then there
-      is unicity of MapsTo. *)
-
-    Lemma Equal_refl : forall m, Sort m -> Equal m m.
-      intros m sorted.
-      unfold Equal.
-      intros e e' e''.
-      split. split;auto.
-      unfold MapsTo.
-      intros mapsto1 mapsto2.
-      induction mapsto1.
-
-      inversion mapsto2.
-      destruct y.
-      unfold eq_key_elt in H1,H; simpl in H1,H.
-      intuition congruence.
-
-      destruct y.
-      subst.      
-      dec_eq_key_elt; simpl in *.
-      absurd (E.eq e k);auto.
-      eapply sorted_in_cons_not_eq with l e0;eauto.
-
-      apply IHmapsto1;eauto.
-      inversion mapsto2;try assumption.
-      destruct y.
-      dec_eq_key_elt; simpl in *.
-      absurd (E.eq e k); auto.
-      eapply sorted_in_cons_not_eq with l e0;eauto.
-    Qed.
-
-Ltac Equal_inv m x e e' := 
-  assert (_Equal_hyp: Equal m m);
-    [ apply Equal_refl;assumption
-  | unfold Equal in _Equal_hyp;elim (_Equal_hyp x e e')
-  ].
-
-    Lemma MapsTo_sorted_eq_elt :  forall k m e e', Sort m -> MapsTo k e m 
-      -> MapsTo k e' m -> e = e'.
-      intros x m e e' sorted.
-      Equal_inv m x e e'. (* m is sorted, so MapsTo is unique modulo eq_elt *)
-      auto.
-    Qed.
-*)
-
-
-      (** Specification of [equal] *) 
-      Variable fcompare: elt->elt->bool.
-      Variable fcompare_ok1:forall e e', fcompare e e' = true -> eq_elt e e'.
-      Variable fcompare_ok2:forall e e', fcompare e e' = false -> ~eq_elt e e'.
-
-      Fixpoint equal (s : t elt) {struct s} : t elt -> bool :=
-	fun s' : t elt =>
-	  match s, s' with
-	    | [], [] => true
-	    | (k,x) :: l, (k',x') :: l' =>
-              match E.compare k k' with
-		| FSetInterface.Eq _ => if fcompare x x' then equal l l' else false
-		| _ => false
-              end
-	    | _, _ => false
-	  end.
-
-       
-      Axiom XXX: forall x e l, In x l -> In x (e::l).
-      Axiom YYY: forall a k x l, (In a ((k, x) :: l)) -> ~E.eq a k -> (In a l).
-
-      Lemma InList_eq_key : forall x x' l,
-	InList eq_key x l -> eq_key x x' -> InList eq_key x' l.
-	intros x x' l H H0.
-	induction H;eauto.
-      Qed.
-	
-
-      Lemma unique_in_eq_key : forall x x' l, Unique eq_key (x'::l)
-	-> InList eq_key_elt x (x'::l) -> eq_key x x' -> eq_key_elt x x'.
-	intros x x' l uniq inl eqk.
-	inversion inl;auto.
-	subst.
-	inversion uniq.
-	elim H2.
-	assert ( inl2 : InList eq_key x l );auto.
-	eapply InList_eq_key with x;auto.
-      Qed.
-
-      Lemma unique_in_eq_key2 : forall x x' l, Unique eq_key l
-	-> InList eq_key_elt x l -> InList eq_key_elt x' l 
-	-> eq_key x x' -> eq_key_elt x x'.
-	intros x x' l uniq inl1 inl2 eqk.
-	induction inl1.
-	inversion inl2.
-	eauto.
-	absurd (InList eq_key y l).
-	inversion uniq.
-	assumption.
-
-	subst.
-	eapply InList_eq_key with x'. auto. eauto.
-
-	apply IHinl1.
-	inversion uniq;auto.
-	eapply aux'' with y;auto.
-	intro abs.
-	absurd (InList eq_key x' l);eauto 5.
-	2: eapply InList_eq_key with x;auto.
-	intro abs2.
-	inversion uniq.
-	elim H1.
-	eapply InList_eq_key with x';auto.
-      Qed.
-
-
-      Lemma ZZZ : forall a e e' l, 
-	Unique eq_key l -> MapsTo a e l -> MapsTo a e' l -> eq_elt e e'.
-	unfold MapsTo,mapsto.
-	intros a e e' l sorted inl1 inl2.
-
-(*
-	assert (Unique eq_key l). apply sorted_unique;auto. *)
-	induction sorted.
-	inversion inl1. 
-
-	elim (@In_inv3 (a, e) x l);auto;intro hyp.
-	assert (eq2:eq_key_elt (a, e) (a,e')).
-	eapply eq_key_elt_trans with x;auto.
-	apply eq_key_elt_sym.
-	eapply unique_in_eq_key with l;auto.
-	simpl in hyp.
-	destruct x;intuition.
-	simpl in eq2;intuition.
-
-	assert ( eqk : eq_key_elt (a,e) (a,e'));try (simpl in *;intuition;fail).
-	eapply unique_in_eq_key2 with (x::l);simpl;eauto.
-      Qed.	
-
-
-      Lemma equal_1 : forall m m', Sort m -> Sort m' 
-	-> Equal eq_elt m m' -> equal m m' = true.
-	intros m m'. unfold Equal.
-	functional induction equal m m';simpl;auto;subst
-	  ; intros sorted1 sorted2 big
-	    ; [destruct t0 as [k x];elim (big k x x) |elim (big k x x)|elim (big k x x)
-
-	      |apply H;eauto;clear H;intros a e' e'';elim(big a e' e'')
-
-	      |elim (big k x x')|elim (big k' x x)];clear big
-	      ; try (intros hyp1 hyp2;elim hyp1 ; clear hyp1; intros in1 in2).
-
-
-	absurd (In k []);eauto. 
-	absurd (In k []);eauto.
-	absurd (In k ((k', x') :: l')).
-	eapply sort_lt_notin with x;auto. 
-	eauto.
-
-	split.
-	split.
-	intro inal.
-	assert (noteqak : ~ E.eq a k).
-	eapply sorted_in_cons_not_eq with l x;auto.
-
-	assert (In a ((k', x') :: l')).
-	apply in1.
-	apply XXX;auto.
-	eapply YYY with k' x';auto.
-	intro abs.
-	elim noteqak; eauto.
-
-	intro inal'.
-	assert (noteqak : ~ E.eq a k').
-	eapply sorted_in_cons_not_eq with l' x';auto.
-	assert (In a ((k, x) :: l)).
-	apply in2.
-	apply XXX;auto.
-	eapply YYY with k x;auto.
-	intro abs.
-	elim noteqak; eauto.
-
-	intros mapsto1 mapsto2.
-	apply hyp2;auto.
-
-	absurd (eq_elt x x');auto 6.
-	
-	absurd (In k' ((k, x) :: l)).
-	eapply sort_lt_notin with x';auto.
-	eauto.
-      Qed.
-
-
-      Lemma equal_2 :forall m m', Sort m -> Sort m' -> 
-	equal m m' = true -> Equal eq_elt m m.
-	intros m m'. unfold Equal.
-      	functional induction equal m m';simpl;auto;subst;intro eq1;auto
-	  ; intros hyp hyp2 a e' e''; try (inversion hyp2;fail)
-	    ;(split;[split;auto|]);intros H1 H2. 
-	inversion H1.
-	eapply ZZZ with a ((k, x) :: l);auto.
-        apply sorted_unique;auto.
-      Qed.
-
-
-
-
-
-
-
-
-
-
-
-
-
-
-
-
-
-
-
-
-Axiom eq: nat -> nat -> Prop.
-Axiom eqall: forall n m:nat, eq n m.
-Definition lt := Peano.lt.
-Axiom eq_refl : forall x : nat, eq x x.
-Axiom eq_sym : forall x y : nat, eq x y -> eq y x.
-Axiom eq_trans : forall x y z : nat, eq x y -> eq y z -> eq x z.
-
-Axiom lt_trans : forall x y z : nat, lt x y -> lt y z -> lt x z.
-Axiom lt_not_eq : forall x y : nat, lt x y -> ~ eq x y.
-
-Require Import Compare_dec.
-Require Import Arith.
-Require Import Le.
-Require Import Lt.
-Module A : OrderedType.
-  Definition t := nat.
-
-
-  Definition compare : forall x y : nat, Compare lt eq x y.
-    intros n m.
-    assert ({n < m} + {n = m} + {m < n}).
-    apply lt_eq_lt_dec.
-    destruct H.
-    destruct s.
-    apply Lt. 
-    assumption.
-    apply Eq. 
-    apply eqall.
-    apply Gt.
-    assumption.
+Module Make_ord (X: OrderedType)(Data : OrderedType) <: 
+    Sord with Module Data := Data with Module MapS.E := X.
+
+  Module Data := Data.
+  Module MapS := Make(X). 
+  Import MapS.
+
+  Module MD := OrderedTypeFacts(Data).
+  Import MD.
+
+  Definition t := MapS.t Data.t. 
+
+  Definition cmp e e' := match Data.compare e e' with Eq _ => true | _ => false end.	
+
+  Fixpoint eq_list (m m' : list (X.t * Data.t)) { struct m } : Prop := 
+       match m, m' with 
+        | [], [] => True
+        | (x,e)::l, (x',e')::l' => 
+            match X.compare x x' with 
+             | Eq _ => Data.eq e e' /\ eq_list l l'
+             | _       => False
+            end 
+        | _, _ => False
+       end.
+
+  Definition eq m m' := eq_list m.(this) m'.(this).
+
+  Fixpoint lt_list (m m' : list (X.t * Data.t)) {struct m} : Prop := match m, m' with 
+    | [], [] => False
+    | [], _  => True
+    | _, []  => False
+    | (x,e)::l, (x',e')::l' => 
+        match X.compare x x' with 
+          | Lt _ => True
+          | Gt _ => False
+          | Eq _ => Data.lt e e' \/ (Data.eq e e' /\ lt_list l l')
+        end
+    end.
+
+  Definition lt m m' := lt_list m.(this) m'.(this).
+
+  Lemma eq_equal : forall m m', eq m m' <-> equal cmp m m' = true.
+  Proof.
+  intros (l,Hl); induction l.
+  intros (l',Hl'); unfold eq; simpl.
+  destruct l'; unfold equal; simpl; intuition.
+  intros (l',Hl'); unfold eq.
+  destruct l'.
+  destruct a; unfold equal; simpl; intuition.
+  destruct a as (x,e).
+  destruct p as (x',e').
+  unfold equal; simpl. 
+  unfold Raw.E.compare.
+  unfold E.compare.
+  destruct (X.compare x x'); simpl; intuition.
+  unfold cmp at 1. 
+  destruct (Data.compare e e'); simpl; intuition. 
+  absurd (Data.lt e e'); eauto.
+  inversion_clear Hl.
+  inversion_clear Hl'.
+  destruct (IHl H (Build_slist H3)).
+  unfold equal, eq in H5; simpl in H5; auto.
+  absurd (Data.lt e' e); eauto.
+  unfold cmp in H; destruct (Data.compare e e'); simpl in H; auto; discriminate.
+  destruct (andb_prop _ _ H); clear H.
+  inversion_clear Hl.
+  inversion_clear Hl'.
+  destruct (IHl H (Build_slist H3)).
+  unfold equal, eq in H6; simpl in H6; auto.
+ Qed.
+
+  Lemma eq_1 : forall m m', Equal cmp m m' -> eq m m'.
+  intros.
+  generalize (@equal_1 Data.t m m' cmp).
+  generalize (@eq_equal m m').
+  intuition.
   Qed.
 
+  Lemma eq_2 : forall m m', eq m m' -> Equal cmp m m'.
+  intros.
+  generalize (@equal_2 Data.t m m' cmp).
+  generalize (@eq_equal m m').
+  intuition.
+  Qed.
 
+  Lemma eq_refl : forall m : t, eq m m.
+  Proof.
+     intros (m,Hm); induction m; unfold eq; simpl; auto.
+     destruct a.
+     destruct (X.compare t0 t0); auto.
+     apply (MapS.Raw.ME.lt_antirefl l); auto.
+     split.
+     apply Data.eq_refl.
+     inversion_clear Hm.
+     apply (IHm H).
+     apply (MapS.Raw.ME.lt_antirefl l); auto.
+  Qed.
 
-  
+  Lemma  eq_sym : forall m1 m2 : t, eq m1 m2 -> eq m2 m1.
+  Proof.
+     intros (m,Hm); induction m; 
+     intros (m', Hm'); destruct m'; unfold eq; simpl;
+     try destruct a as (x,e); try destruct p as (x',e'); auto.
+     destruct (X.compare x x'); destruct (X.compare x' x); intuition; 
+      try solve [absurd (X.eq x x'); eauto]. 
+     inversion_clear Hm; inversion_clear Hm'.
+     apply (IHm H (Build_slist H3)); auto.
+  Qed.
 
+  Lemma eq_trans : forall m1 m2 m3 : t, eq m1 m2 -> eq m2 m3 -> eq m1 m3.
+     intros (m1,Hm1); induction m1; 
+     intros (m2, Hm2); destruct m2; 
+     intros (m3, Hm3); destruct m3; unfold eq; simpl; 
+     try destruct a as (x,e); 
+     try destruct p as (x',e'); 
+     try destruct p0 as (x'',e''); try contradiction; auto.
+     destruct (X.compare x x'); 
+       destruct (X.compare x' x''); 
+         destruct (X.compare x x''); intros; auto; 
+            try solve [ contradiction | 
+                            absurd (X.lt x x''); eauto | 
+                            absurd (X.lt x' x''); eauto | 
+                            absurd (X.lt x'' x'); eauto ].
+    split; intuition eauto.
+     inversion_clear Hm1; inversion_clear Hm2; inversion_clear Hm3.
+     apply (IHm1 H0 (Build_slist H5) (Build_slist H7)); intuition.
+   Qed.
 
-  Definition eq := eq.
-  Definition lt := lt.
-  Definition eq_refl:= eq_refl.
-  Definition eq_sym:= eq_sym.
-  Definition eq_trans:= eq_trans.
-  Definition lt_trans:= lt_trans.
-  Definition lt_not_eq:= lt_not_eq.
-End A.
+  Lemma lt_trans : forall m1 m2 m3 : t, lt m1 m2 -> lt m2 m3 -> lt m1 m3.
+  Proof.
+     intros (m1,Hm1); induction m1; 
+     intros (m2, Hm2); destruct m2; 
+     intros (m3, Hm3); destruct m3; unfold lt; simpl; 
+     try destruct a as (x,e); 
+     try destruct p as (x',e'); 
+     try destruct p0 as (x'',e''); try contradiction; auto.
+     destruct (X.compare x x'); 
+       destruct (X.compare x' x''); 
+         destruct (X.compare x x''); intros; auto; 
+            try solve [ contradiction | 
+                            absurd (X.lt x x''); eauto | 
+                            absurd (X.lt x' x''); eauto | 
+                            absurd (X.lt x'' x'); eauto ].
+    intuition; try solve [left; eauto].
+    right. 
+    split; eauto.
+     inversion_clear Hm1; inversion_clear Hm2; inversion_clear Hm3.
+     apply (IHm1 H1 (Build_slist H5) (Build_slist H7)); intuition.
+   Qed.
 
-Module B : S with Module E:=A.
+  Lemma lt_not_eq : forall m1 m2 : t, lt m1 m2 -> ~ eq m1 m2.
+     intros (m1,Hm1); induction m1; 
+     intros (m2, Hm2); destruct m2; unfold eq, lt; simpl; 
+     try destruct a as (x,e); 
+     try destruct p as (x',e'); try contradiction; auto.
+     destruct (X.compare x x'); auto.
+     intuition.
+     absurd (Data.lt e e'); eauto.
+     inversion_clear Hm1; inversion_clear Hm2.
+     apply (IHm1 H0 (Build_slist H5)); intuition.
+   Qed.
 
+  Definition compare : forall m1 m2, Compare lt eq m1 m2.
+    intros (m1,Hm1); induction m1; 
+    intros (m2, Hm2); destruct m2.
+    apply Eq; unfold eq; simpl; auto.
+    apply Lt; unfold lt; simpl; auto.
+    apply Gt; unfold lt; simpl; auto. 
+    destruct a as (x,e); destruct p as (x',e'). 
+    destruct (X.compare x x').
+    apply Lt; unfold lt; simpl; 
+     destruct (X.compare x x'); auto; absurd (X.lt x x'); eauto.
+    destruct (Data.compare e e').
+    apply Lt; unfold lt; simpl;
+     destruct (X.compare x x'); auto; absurd (X.eq x x'); eauto.
+    assert (Hm11 : sort (Raw.lt_key (elt:=Data.t)) m1).
+     inversion_clear Hm1; auto.
+    assert (Hm22 : sort (Raw.lt_key (elt:=Data.t)) m2).
+     inversion_clear Hm2; auto.
+    destruct (IHm1 Hm11 (Build_slist Hm22)).
+    apply Lt; unfold lt; simpl; 
+      destruct (X.compare x x'); try (right; auto); absurd (X.eq x x'); eauto.
+    apply Eq; unfold eq; simpl; 
+       destruct (X.compare x x'); auto; absurd (X.eq x x'); eauto.
+    apply Gt; unfold lt; simpl;
+     destruct (X.compare x' x); auto; absurd (X.eq x x'); eauto.
+    apply Gt; unfold lt; simpl;
+     destruct (X.compare x' x); auto; absurd (X.eq x x'); eauto.
+    apply Gt; unfold lt; simpl;
+     destruct (X.compare x' x); auto; absurd (X.lt x' x); eauto.
+    Qed.
 
-  Eval compute in (Raw.equal ((1,23)::(2,34)::[]) ((1,23)::(2,34)::[])).
-
-*)
+End Make_ord. 
